updating meta-F* playground to show of CL style , and #. !!!

Fstar/fun/Meta/First.fst
@@ -1,6 +1,23 @@
 module First
 
 open FStar.Tactics
+open FStar.Tactics.Derived
+
+
+(**** Meta I came up with myself *)
+
+let add_1_generator () : Tac unit =
+  let x = intro () in
+  let tm = (`(`#x + `@1)) in
+  apply tm
+
+val add_1 : int -> int
+let add_1 = _ by (add_1_generator ())
+
+
+
+(**** Meta I found online *)
+
 
 val id (#a : Type) : a -> a
 let id  =
@@ -12,4 +29,43 @@ let id  =
 
 let test'' = id 3
 
-let t' = `(0 + 1)
+let t' x = `(0 + 1 ,x)
+let t'' = t' 2
+
+let f (x y : int) : int = _ by (exact (`42))
+
+let mk_add () : Tac unit =
+  let x = intro () in
+  let y = intro () in
+  apply (`(+));
+  exact y;
+  exact x
+
+let add : int -> int -> int =
+  _ by (mk_add ())
+
+
+type t1 =
+  | A : int -> int -> t1
+  | B : string -> t1
+  | C : t1 -> t1
+
+// let t1_print : t1 -> string = _ by ( ())
+
+(* interesting to note is that we can `@z here *)
+let _ = assert True
+            by (let tm = (`(1 + `@(1))) in
+                let z = 16 in
+                let x = `16 in
+                let tm2 = `(1 + `@(z)) in
+                let tm3 = `(1 + `#(x)) in
+                debug ("tm = " ^ term_to_string tm);
+                debug ("tm2 = " ^ term_to_string tm2);
+                debug ("tm3 = " ^ term_to_string tm3);
+                let ty = tc (cur_env ()) tm in
+                debug ("ty = " ^ term_to_string ty);
+                let ty2 = tc (cur_env ()) tm2 in
+                debug ("ty2 = " ^ term_to_string ty2);
+                let ty3 = tc (cur_env ()) tm3 in
+                debug ("ty3 = " ^ term_to_string ty3);
+                ())
